src/Spec/PointEncoding.v
@@ -6,22 +6,21 @@ Require Crypto.ModularArithmetic.PrimeFieldTheorems.
 Require Bedrock.Word.
 Require Crypto.Tactics.VerdiTactics.
 Require Crypto.Encoding.PointEncodingPre.
-Obligation Tactic := eauto using PointEncodingPre.point_encoding_canonical.
+Obligation Tactic := eauto; exact PointEncodingPre.point_encoding_canonical.
 
-Require Import Crypto.Spec.Encoding Crypto.Spec.ModularArithmetic.
-Require Import Crypto.Spec.CompleteEdwardsCurve.
+Require Import Crypto.Spec.Encoding Crypto.Spec.ModularWordEncoding.
+Require Import Crypto.Spec.CompleteEdwardsCurve Crypto.Spec.ModularArithmetic.
 
 Local Open Scope F_scope.
 
 Section PointEncoding.
-  Context {prm: CompleteEdwardsCurve.TwistedEdwardsParams} {sz : nat}
-   {FqEncoding : encoding of ModularArithmetic.F (CompleteEdwardsCurve.q) as Word.word sz}.
-
-  Definition sign_bit (x : F CompleteEdwardsCurve.q) :=
-    match (enc x) with
-      | Word.WO => false
-      | Word.WS b _ w' => b
-    end.
+  Context {prm: TwistedEdwardsParams} {sz : nat} {sz_nonzero : (0 < sz)%nat}
+   {bound_check : (BinInt.Z.to_nat q < NPeano.Nat.pow 2 sz)%nat} {q_5mod8 : (q mod 8 = 5)%Z}
+   {sqrt_minus1_valid : (@ZToField q 2 ^ BinInt.Z.to_N (q / 4)) ^ 2 = opp 1}
+   {FqEncoding : encoding of (F q) as (Word.word sz)}
+   {sign_bit : F q -> bool} {sign_bit_zero : sign_bit 0 = false}
+   {sign_bit_opp : forall x, x <> 0 -> negb (sign_bit x) = sign_bit (opp x)}.
+  Existing Instance prime_q.
 
   Definition point_enc (p : E.point) : Word.word (S sz) := let '(x,y) := proj1_sig p in
     Word.WS (sign_bit x) (enc y).
@@ -29,13 +28,20 @@ Section PointEncoding.
   Program Definition point_dec_with_spec :
     {point_dec : Word.word (S sz) -> option E.point
                | forall w x, point_dec w = Some x -> (point_enc x = w)
-               } := PointEncodingPre.point_dec.
-   
+               } := @PointEncodingPre.point_dec _ _ _ sign_bit.
+
   Definition point_dec := Eval hnf in (proj1_sig point_dec_with_spec).
+
+   Definition point_encoding_valid : forall p : E.point, point_dec (point_enc p) = Some p :=
+     @PointEncodingPre.point_encoding_valid _ _ sz_nonzero bound_check q_5mod8 sqrt_minus1_valid _ _ sign_bit_zero sign_bit_opp.
+
+   Definition point_encoding_canonical : forall x_enc x, point_dec x_enc = Some x -> point_enc x = x_enc :=
+     PointEncodingPre.point_encoding_canonical . 
 
   Instance point_encoding : encoding of E.point as (Word.word (S sz)) := {
     enc := point_enc;
     dec := point_dec;
-    encoding_valid := PointEncodingPre.point_encoding_valid
+    encoding_valid := point_encoding_valid;
+    encoding_canonical := point_encoding_canonical
   }.
 End PointEncoding.
