src/Encoding/ModularWordEncodingTheorems.v
@@ -1,0 +1,89 @@
+Require Import Coq.ZArith.ZArith Coq.ZArith.Znumtheory.
+Require Import Coq.Numbers.Natural.Peano.NPeano.
+Require Import Crypto.CompleteEdwardsCurve.CompleteEdwardsCurveTheorems.
+Require Import Crypto.ModularArithmetic.PrimeFieldTheorems.
+Require Import Bedrock.Word.
+Require Import Crypto.Tactics.VerdiTactics.
+Require Import Crypto.Spec.Encoding.
+Require Import Crypto.Spec.ModularWordEncoding.
+
+
+Local Open Scope F_scope.
+
+Section SignBit.
+  Context {m : Z} {prime_m : prime m} {two_lt_m : (2 < m)%Z} {sz : nat} {bound_check : (Z.to_nat m < 2 ^ sz)%nat}.
+  Lemma m_pos : (0 < m)%Z.
+  Proof.
+    apply prime_ge_2 in prime_m; omega.
+  Qed.
+
+  Arguments modular_word_encoding {m} {sz} m_pos bound_check.
+  Let Fm_encoding := modular_word_encoding m_pos bound_check.
+
+  Definition sign_bit (x : F m) :=
+  match (@enc _ _ Fm_encoding x) with
+    | Word.WO => false
+    | Word.WS b _ w' => b
+  end.
+
+  Lemma sign_bit_parity : forall x, sign_bit x = Z.odd x.
+  Proof.
+    unfold sign_bit; intros.
+    unfold Fm_encoding, enc, modular_word_encoding, Fm_enc.
+    pose proof (shatter_word (NToWord sz (Z.to_N x))) as shatter.
+    case_eq sz; intros; subst; rewrite shatter.
+    + pose proof (prime_ge_2 m prime_m).
+      simpl in bound_check.
+      assert (m < 1)%Z by (apply Z2Nat.inj_lt; try omega; assumption).
+      omega.
+    + pose proof (FieldToZ_range x m_pos).  
+      destruct (FieldToZ x); auto.
+      - destruct p; auto.
+      - pose proof (Pos2Z.neg_is_neg p); omega.
+   Qed.
+
+  Lemma sign_bit_zero : sign_bit 0 = false.
+  Proof.
+    rewrite sign_bit_parity; auto.
+  Qed.
+
+  (* TODO : move to ZUtil *)
+  Lemma Z_odd_mod : forall a b, (b <> 0)%Z ->
+    Z.odd (a mod b) = if Z.odd b then xorb (Z.odd a) (Z.odd (a / b)) else Z.odd a.
+  Proof.
+    intros.
+    rewrite Zmod_eq_full by assumption.
+    rewrite <-Z.add_opp_r, Z.odd_add, Z.odd_opp, Z.odd_mul.
+    break_if; rewrite ?Bool.andb_true_r, ?Bool.andb_false_r; auto using Bool.xorb_false_r.
+  Qed.
+
+  (* TODO : move to ModularArithmeticTheorems *)
+  Lemma F_FieldToZ_add_opp : forall x : F m, x <> 0 -> (FieldToZ x + FieldToZ (opp x) = m)%Z.
+  Proof.
+    intros.
+    rewrite FieldToZ_opp.
+    rewrite Z_mod_nz_opp_full, mod_FieldToZ; try omega.
+    rewrite mod_FieldToZ.
+    replace 0%Z with (@FieldToZ m 0) by auto.
+    intro false_eq.
+    rewrite <-F_eq in false_eq.
+    congruence.
+  Qed.
+
+  Lemma sign_bit_opp : forall (x : F m), x <> 0 -> negb (sign_bit x) = sign_bit (opp x).
+  Proof.
+    intros.
+    pose proof sign_bit_zero as sign_zero.
+    rewrite !sign_bit_parity in *.
+    pose proof (F_opp_spec x) as opp_spec_x.
+    apply F_eq in opp_spec_x.
+    rewrite FieldToZ_add in opp_spec_x.
+    rewrite <-opp_spec_x, Z_odd_mod in sign_zero by omega.
+    replace (Z.odd m) with true in sign_zero by (destruct (ZUtil.prime_odd_or_2 m prime_m); auto || omega).
+    rewrite Z.odd_add, F_FieldToZ_add_opp, Z.div_same, Bool.xorb_true_r in sign_zero by assumption || omega.
+    apply Bool.xorb_eq.
+    rewrite <-Bool.negb_xorb_l.
+    assumption.
+  Qed.
+
+End SignBit.
